SELFOUR-276: Prove refinement to Haskell for MCP
Also includes fixes to specs and invariants, and initial progress
towards C refinement.

A thread's maximum controlled priority (MCP) determines the maximum
thread priority or MCP it can assign to another thread (or itself).

spec/haskell/src/SEL4/API/Types.lhs
@@ -140,8 +140,8 @@ The priority of a thread is represented by an 8-bit unsigned integer.
 
 > prioPropsFromWord :: Word -> PrioProps
 > prioPropsFromWord w = PrioProps {
->         ppPriority = fromIntegral $ toInteger $ w .&. (bit priorityBits - 1),
->         ppMCP = fromIntegral $ toInteger $ (w `shiftR` priorityBits) .&. (bit mcpBits - 1)}
+>         ppPriority =  fromIntegral $ w .&. mask priorityBits,
+>         ppMCP = fromIntegral $ (w `shiftR` priorityBits) .&. (mask mcpBits)}
 
 \subsection{Capability References}
 
