spec/abstract/Decode_A.thy
@@ -213,21 +213,21 @@ where
 
 
 definition check_prio
-  :: "priority \<Rightarrow> obj_ref \<Rightarrow> (unit,'z::state_ext) se_monad" where
-  "check_prio new_prio cur \<equiv>
-    do
-      mcp \<leftarrow> thread_get tcb_mcpriority cur;
+  :: "priority \<Rightarrow> (unit,'z::state_ext) se_monad" where
+  "check_prio new_prio \<equiv>
+    doE
+      cur \<leftarrow> liftE $ gets cur_thread;
+      mcp \<leftarrow> liftE $ thread_get tcb_mcpriority cur;
       whenE (new_prio > mcp) $ throwError (RangeError 0 (ucast mcp))      
-    od"
+    odE"
+    
 definition check_mcp
-  :: "priority \<Rightarrow> obj_ref \<Rightarrow> (unit,'z::state_ext) se_monad" where
-  "check_mcp new_mcp cur \<equiv>
-    do
-      mcp \<leftarrow> thread_get tcb_mcpriority cur;
-      check_prio mcp cur;
+  :: "priority \<Rightarrow> (unit,'z::state_ext) se_monad" where
+  "check_mcp new_mcp \<equiv>
+    doE
+      check_prio new_mcp;
       whenE (new_mcp > maxPrio) $ throwError (RangeError 0 (ucast maxPrio))
-    od"    
-
+    odE"    
 
 definition
   decode_set_priority :: "data list \<Rightarrow> cap \<Rightarrow> cslot_ptr \<Rightarrow> (tcb_invocation,'z::state_ext) se_monad"
@@ -235,21 +235,20 @@ where
   "decode_set_priority args cap slot \<equiv> 
      if length args = 0 then throwError TruncatedMessage
      else let prio = (ucast $ args ! 0) in doE
-       cur \<leftarrow> liftE $ gets cur_thread;
-       check_prio prio cur;
+       check_prio prio;
        returnOk (ThreadControl (obj_ref_of cap) slot None
-             (Some prio) None None None None)
+             None (Some prio) None None None)
     odE"
+    
 definition
   decode_set_mcpriority :: "data list \<Rightarrow> cap \<Rightarrow> cslot_ptr \<Rightarrow> (tcb_invocation,'z::state_ext) se_monad"
 where
   "decode_set_mcpriority args cap slot \<equiv> 
      if length args = 0 then throwError TruncatedMessage
      else let new_mcp = ucast $ args ! 0 in doE
-       cur \<leftarrow> liftE $ gets cur_thread;
-       check_mcp new_mcp cur;
+       check_mcp new_mcp;
        returnOk (ThreadControl (obj_ref_of cap) slot None
-             None (Some new_mcp)None None None)
+             (Some new_mcp) None None None None)
      odE"
 
 definition
@@ -310,10 +309,10 @@ where
  odE"
 
 definition prio_from_word :: "data \<Rightarrow> data" where
-"prio_from_word w \<equiv> ucast w"
+"prio_from_word w \<equiv> w && mask 8"
 
 definition mcp_from_word :: "data \<Rightarrow> data" where
-"mcp_from_word w \<equiv> ucast (shiftr w 8)"
+"mcp_from_word w \<equiv> (w >> 8) && mask 8"
 
 
 definition
@@ -335,7 +334,7 @@ where
      set_params \<leftarrow> decode_set_ipc_buffer [buffer] cap slot [buffer_cap];
      set_space \<leftarrow> decode_set_space [fault_ep, croot_data, vroot_data] cap slot crootvroot;
      returnOk $ ThreadControl (obj_ref_of cap) slot (tc_new_fault_ep set_space)
-                              (tc_new_priority set_prio) (tc_new_mcpriority set_mcp)
+                              (tc_new_mcpriority set_mcp) (tc_new_priority set_prio)
                               (tc_new_croot set_space) (tc_new_vroot set_space) 
                               (tc_new_buffer set_params)
    odE" 
